coq/Common/AllDiff.v
@@ -5,8 +5,6 @@ Require Import Coq.Lists.List.
 
 Local Open Scope list_scope.
 
-Print Coq.Lists.List.
-
 Fixpoint AllDiff (A B : Type) (f : A -> B) (lst : list A) : Prop :=
   match lst with
     | nil => True
@@ -35,4 +33,54 @@ Proof with auto with datatypes.
   apply HDiffHd in H0.
   symmetry in H2.
   contradiction.
+Qed.
+
+Lemma map_eq_inj : forall (A B : Type) (f : A -> B) (lst1 lst2 : list A) (x : A),
+  map f lst1 = map f lst2 ->
+  In x lst1 ->
+  exists (y : A),
+    In y lst2 /\ f x = f y.
+Proof with auto with datatypes.
+  intros.
+  generalize dependent lst1.
+  induction lst2; intros.
+  simpl in H. destruct lst1. inversion H0. simpl in H. inversion H.
+  destruct lst1.
+  simpl in H. inversion H0.
+  simpl in H.
+  inversion H.
+  simpl in H0.
+  destruct H0.
+  subst. exists a...
+  apply IHlst2 in H0...
+  destruct H0 as [y0 [HIn2 HEq]].
+  exists y0...
+Qed.
+
+Lemma AllDiff_preservation : forall
+  (A B : Type) (f : A -> B) (lst1 lst2 : list A),
+  AllDiff f lst1 ->
+  map f lst1 = map f lst2 ->
+  AllDiff f lst2.
+Proof with auto with datatypes.
+  intros.
+  generalize dependent lst1.
+  induction lst2; intros.
+  simpl...
+  destruct lst1.
+  simpl in H0. inversion H0.
+  simpl in H0.
+  inversion H0.
+  simpl in H.
+  destruct H as [HDiffHd HDiffTl].
+  simpl.
+  split.
+  intros.
+  apply map_eq_inj with (f := f) (lst2 := lst1) in H...
+  destruct H as [y0 [HIn2 HEqyy0]].
+  apply HDiffHd in HIn2.
+  rewrite -> HEqyy0.
+  rewrite <- H2.
+  trivial.
+  apply IHlst2 in H3...
 Qed.
